Progress on bridging the gap between functional spec and crypto spec

hmacdrbg/HMAC256_DRBG_bridge_to_FCF.v
@@ -14,10 +14,21 @@ Require Import Coqlib.
 Require Import fcf.Fold.
 Import ListNotations.
 
-(* 
-Definition Instantiate (entropy nonce: list Z) : DRBG_functions.DRBG_working_state :=
-HMAC256_DRBG_instantiate_algorithm  entropy nonce nil 0. 
-*)
+Lemma false_zgt z a: false = (z >? a) -> z<=a. 
+Proof. unfold Z.gtb.
+  remember (z ?= a). destruct c. symmetry in Heqc; apply Z.compare_eq in Heqc. subst; intros. omega.
+  symmetry in Heqc. destruct (Z.compare_lt_iff z a); intros. apply H in Heqc. omega.
+  discriminate.
+Qed. 
+Lemma false_zge z a: false = (z >=? a) -> z<a. 
+Proof. unfold Z.geb.
+  remember (z ?= a). destruct c; intros; try discriminate.
+  symmetry in Heqc. destruct (Z.compare_lt_iff z a); intros. apply H0 in Heqc. omega.
+Qed.
+Lemma false_zge' z a (A:z<a): false = (z >=? a). 
+Proof.
+  remember ((z >=? a)). destruct b; trivial. symmetry in Heqb. apply Z.geb_le in Heqb. omega.
+Qed.
 
 Lemma bytesToBits_InBlocks l: InBlocks 8 (bytesToBits l).
 Proof.
@@ -250,19 +261,30 @@ Proof. induction n; simpl; intros.
   split; trivial. 
 Qed.
 
-Definition Equiv n:= forall k v blocks u,
-   Gen_loop_Zlist k v n = (blocks, u) ->
-   HMAC_DRBG_generate_helper_Z HMAC256 k v (32*(Z.of_nat n-1)+1) = (u,flatten (rev blocks)).
+Definition Equiv n:= forall k v blocks u 
+   (G: Gen_loop_Zlist k v n = (blocks, u)) m
+   (M: 32*(Z.of_nat n-1) < m <=32*(Z.of_nat n)),
+   HMAC_DRBG_generate_helper_Z HMAC256 k v m = (u,flatten (rev blocks)).
 
 Lemma E1: Equiv 1.
-Proof. unfold Equiv, HMAC_DRBG_generate_helper_Z; simpl; intros.
-  inv H; simpl. rewrite app_nil_r; trivial. 
+Proof. unfold Equiv. simpl; intros. inv G. simpl. rewrite app_nil_r.
+ rewrite HMAC_DRBG_generate_helper_Z_equation'; try omega. simpl.
+ rewrite HMAC_DRBG_generate_helper_Z_equation.
+ assert (0 >=? m - 32 = true). apply Z.geb_le; omega.
+ rewrite H; trivial.
 Qed.
 
 Lemma E2: Equiv 2.
-Proof. unfold Equiv, HMAC_DRBG_generate_helper_Z; simpl; intros.
-  inv H; simpl. rewrite app_nil_r; trivial. 
-Qed.
+Proof. unfold Equiv; simpl; intros.
+  inv G; simpl.
+ rewrite HMAC_DRBG_generate_helper_Z_equation'; try omega. simpl.
+ rewrite HMAC_DRBG_generate_helper_Z_equation.
+ assert (false = (0 >=? m - 32)) by (apply false_zge'; omega).
+ rewrite <- H. simpl.
+ rewrite HMAC_DRBG_generate_helper_Z_equation.
+ assert ((0 >=? m - 32 - 32)= true) by (apply Z.geb_le; omega).
+ rewrite H0. rewrite app_nil_r; trivial. 
+Qed. (*
 
 Lemma E3: Equiv 3.
 Proof. unfold Equiv, HMAC_DRBG_generate_helper_Z; simpl; intros.
@@ -278,8 +300,8 @@ Lemma E10: Equiv 10.
 Proof. unfold Equiv, HMAC_DRBG_generate_helper_Z; simpl; intros.
   inv H; simpl. rewrite ! app_assoc, app_nil_r; trivial. 
 Qed.
-
-(*Hence, by induction this should be the equivalence property*)
+*)
+(*Hence, by induction the following equivalence property holds*)
 
 Lemma E_aux k: forall n v blocks u,
                Gen_loop_Zlist k (HMAC256 v k) n = (blocks, u) ->
@@ -298,32 +320,35 @@ Proof. induction n; intros.
 Qed.
 
 Lemma E: forall n, Equiv (S n).
-Proof. induction n; unfold Equiv in *; intros.
-+ simpl in *. inv H; subst; unfold HMAC_DRBG_generate_helper_Z; simpl.
-  rewrite app_nil_r; trivial.
-+ remember (S n) as N. simpl in H.
+Proof. induction n.
++ apply E1. 
++ unfold Equiv in *; intros. remember (S n) as N. 
+  simpl in G.
   remember (Gen_loop_Zlist k (HMAC256 v k) N) as p.
-  destruct p; symmetry in Heqp. inv H.
+  destruct p; symmetry in Heqp. inversion G; clear G. subst blocks l0. 
   rewrite HMAC_DRBG_generate_helper_Z_equation'.
-  Focus 2. specialize (Nat2Z.inj_sub (S (S n)) 1). intros Q.
-   replace (Z.of_nat 1) with 1 in Q; trivial. rewrite <- Q; omega.
-  remember (S n) as N. 
-  assert (W: 32 * (Z.of_nat (S N) - 1) + 1 - Z.of_nat 32 =
-          32 * (Z.of_nat N - 1) + 1).
-  { specialize (Nat2Z.inj_sub (S N) 1). intros Q.
-    replace (Z.of_nat 1) with 1 in Q; trivial. rewrite <- Q by omega; clear Q.
-    simpl. rewrite <- minus_n_O, Z.mul_sub_distr_l; omega. }
-  rewrite W; clear W. 
-  apply Gen_loop_Zlist_nestedV' in Heqp.
-  destruct Heqp as [aa [bb [G [X L]]]]; subst. 
-  rewrite (IHn _ _ _ _ G); clear IHn. 
-  simpl. f_equal. rewrite rev_app_distr. 
+  Focus 2. rewrite Zmult_minus_distr_l in M.
+    assert (64 <= 32 * Z.of_nat (S N)).
+    { subst. replace 64 with (32*2) by omega. apply Z.mul_le_mono_nonneg_l. omega.
+      clear. apply (Nat2Z.inj_le 2). omega. }
+    omega.
+  simpl.
+  apply Gen_loop_Zlist_nestedV' in Heqp. 
+  destruct Heqp as [aa [bb [G [X L]]]]. subst u l.
+  rewrite (IHn _ _ _ _ G); clear IHn.
+  Focus 2. clear - M. 
+           rewrite Zmult_minus_distr_l in *. rewrite Nat2Z.inj_succ in M. simpl in *.
+           omega.
+  f_equal. rewrite rev_app_distr. 
 
-  simpl in G. remember (Gen_loop_Zlist k (HMAC256 v k) n).
+  subst N; simpl in G. remember (Gen_loop_Zlist k (HMAC256 v k) n).
   destruct p. inv G. rewrite map_app, ! rev_app_distr, ! flatten_app.
   simpl. rewrite ! app_nil_r, <- app_assoc. f_equal.
   symmetry in Heqp. apply (E_aux k n); trivial.
 Qed.
+
+Lemma EE n (N:(0<n)%nat): Equiv n.
+Proof. destruct n. omega. apply E; trivial. Qed.
 
 Definition GenUpdate_original_core (state : KV 256) (n : nat) :
   (list (Bvector 256) * KV 256) :=
@@ -425,7 +450,25 @@ Definition Generate RI (WS: DRBG_functions.DRBG_working_state) n: DRBG_functions
                                            WS
                                            n
                                            nil.
+Opaque mult. 
 
+Lemma GenerateCorrect RI k v z n (Z: (z<=RI)%Z) (N:(0<n)%nat):
+  match GenUpdate_original_Zlist (k,v) n with (blocks,(k',v')) => 
+    Generate RI (v, k, z) (Z.of_nat ((32 * n)%nat)) = 
+    generate_algorithm_success (firstn ((32 * n)%nat) (fcf.Fold.flatten (rev blocks))) (v',k',(z+1)%Z) 
+  end.
+Proof. remember (GenUpdate_original_Zlist (k, v) n) as p; destruct p as [kk [vv zz]]; symmetry in Heqp. 
+  unfold GenUpdate_original_Zlist in Heqp.
+  remember (Gen_loop_Zlist k v n) as q; destruct q as [blocks v']; symmetry in Heqq; inv Heqp.
+  apply EE in Heqq; trivial. remember (Z.of_nat (32 * n)) as a.  
+  simpl. remember (z >? RI) as d. destruct d; symmetry in Heqd. 
+  + apply Zgt_is_gt_bool in Heqd; omega.
+  + rewrite Z.mul_sub_distr_l in Heqq. 
+    rewrite Heqq. subst a; rewrite Nat2Z.id; trivial.
+    subst a; clear -N. simpl. rewrite Nat2Z.inj_mul. simpl; omega.
+Qed.
+Opaque Generate.
+(*
 Lemma GenerateCorrect RI k v z n (Z: (z<=RI)%Z):
   match GenUpdate_original_Zlist (k,v) (S n) with (blocks,(k',v')) => 
     Generate RI (v, k, z) (Z.of_nat ((32 * n +1)%nat)) = 
@@ -443,7 +486,21 @@ Proof. remember (GenUpdate_original_Zlist (k, v) (S n)) as p; destruct p as [kk 
       rewrite Z.mul_add_distr_l, Nat2Z.inj_mul. simpl; omega. }
     rewrite W in Heqq. rewrite Heqq, Nat2Z.id; trivial.
 Qed.
-
+*)
+Lemma Generate_Blist_ok RI k v z n (Z: (z<=RI)%Z) l kk vv zz 
+    (K: Forall isbyteZ k) (V:Forall isbyteZ v) (N:(0<n)%nat):
+    Generate RI (v, k, z) (Z.of_nat ((32 * n)%nat)) = generate_algorithm_success l (kk,vv, zz) ->
+    exists y,
+    GenUpdate_original_Blist (bytesToBits k, bytesToBits v) n = 
+    (map bytesToBits y,(bytesToBits vv, bytesToBits kk)) /\ zz=z+1 /\ 
+    l = firstn (32 * n) (flatten (rev y)).
+Proof.
+  remember (GenUpdate_original_Zlist (k,v) n) as g. symmetry in Heqg; destruct g as [a [b c]].
+  specialize (GenerateCorrect RI k v z n Z N). rewrite Heqg; intros HH1 HH2.
+  rewrite HH1 in HH2. exists a. inv HH2. repeat split; trivial. 
+  specialize (GenUpdate_original_Zlist_Blist k v n K V).
+  rewrite Heqg; intros HH; rewrite HH; trivial.
+Qed. (*
 Lemma Generate_Blist_ok RI k v z n (Z: (z<=RI)%Z) l kk vv zz 
     (K: Forall isbyteZ k) (V:Forall isbyteZ v):
     Generate RI (v, k, z) (Z.of_nat ((32 * n +1)%nat)) = generate_algorithm_success l (kk,vv, zz) ->
@@ -457,28 +514,28 @@ Proof.
   rewrite HH1 in HH2. exists a. inv HH2. repeat split; trivial. 
   specialize (GenUpdate_original_Zlist_Blist k v (S n) K V).
   rewrite Heqg; intros HH; rewrite HH; trivial.
-Qed.
+Qed.*)
 
-Lemma Generate_Bvec_ok' RI k v z n (Z: (z<=RI)%Z) l kk vv zz 
+Lemma Generate_Bvec_ok' RI k v z n (Z: (z<=RI)%Z) l kk vv zz (N:(0<n)%nat)
     (K: Forall isbyteZ k) (KL: length (bytesToBits k) = 256%nat) (V:Forall isbyteZ v) (VL:length (bytesToBits v) = 256%nat):
-    Generate RI (v, k, z) (Z.of_nat ((32 * n +1)%nat)) = generate_algorithm_success l (kk,vv, zz) ->
-    match GenUpdate_original_Bvec (of_list_length _ KL, of_list_length _ VL) (S n) with (blocks, kv) =>
+    Generate RI (v, k, z) (Z.of_nat ((32 * n)%nat)) = generate_algorithm_success l (kk,vv, zz) ->
+    match GenUpdate_original_Bvec (of_list_length _ KL, of_list_length _ VL) n with (blocks, kv) =>
     zz=z+1 /\ 
     bitsToBytes (@Vector.to_list _ 256 (fst kv)) = vv /\ 
     bitsToBytes (@Vector.to_list _ 256 (snd kv)) = kk /\
-          l = firstn (32 * n + 1) (bitsToBytes (flatten (rev (map (@Vector.to_list _ 256) blocks))))
+          l = firstn (32 * n) (bitsToBytes (flatten (rev (map (@Vector.to_list _ 256) blocks))))
     end.
 Proof.
-  remember (GenUpdate_original_Zlist (k,v) (S n)) as g. symmetry in Heqg; destruct g as [a [b c]].
-  specialize (GenerateCorrect RI k v z n Z). rewrite Heqg; intros HH1 HH2.
-  rewrite HH1 in HH2. Opaque mult. inv HH2. 
-  specialize (GenUpdate_original_Zlist_Blist k v (S n) K V).
+  remember (GenUpdate_original_Zlist (k,v) n) as g. symmetry in Heqg; destruct g as [a [b c]].
+  specialize (GenerateCorrect RI k v z n Z N). rewrite Heqg; intros HH1 HH2.
+  rewrite HH1 in HH2. inv HH2. 
+  specialize (GenUpdate_original_Zlist_Blist k v n K V).
   rewrite Heqg. intros HH.
   specialize (GenUpdate_original_Blist_Bvec (of_list_length (bytesToBits k) KL)
-                (of_list_length (bytesToBits v) VL) (S n)); intros X. 
+                (of_list_length (bytesToBits v) VL) n); intros X. 
   remember (GenUpdate_original_Bvec
-    (of_list_length (bytesToBits k) KL, of_list_length (bytesToBits v) VL)
-    (S n)) as w. destruct w; symmetry in Heqw.
+    (of_list_length (bytesToBits k) KL, of_list_length (bytesToBits v) VL) n) as w.
+  destruct w; symmetry in Heqw.
   simpl in X. simpl in Heqw. rewrite Heqw in X; clear Heqw.
   destruct k0 as [w u]. rewrite ! HMAC_equivalence.of_length_proof_irrel in X.
   simpl in HH. rewrite HH in X; clear HH. inv X. split. trivial. simpl.
@@ -487,23 +544,23 @@ Proof.
   repeat split; trivial.
   rewrite <- map_rev. f_equal. apply flatten_bytes_bits. apply Forall_rev; trivial.
 Qed.
-Lemma Generate_Bvec_ok RI k v z n (Z: (z<=RI)%Z) 
+Lemma Generate_Bvec_ok RI k v z n (Z: (z<=RI)%Z) (N:(0<n)%nat)
               (K: Forall isbyteZ k) (KL: length (bytesToBits k) = 256%nat)
               (V:Forall isbyteZ v) (VL:length (bytesToBits v) = 256%nat):
-    match GenUpdate_original_Bvec (of_list_length _ KL, of_list_length _ VL) (S n) with (blocks, (kk,vv)) =>
-          Generate RI (v, k, z) (Z.of_nat ((32 * n +1)%nat)) 
-          = generate_algorithm_success (firstn (32 * n + 1) (bitsToBytes (flatten (rev (map (@Vector.to_list _ 256) blocks)))))
+    match GenUpdate_original_Bvec (of_list_length _ KL, of_list_length _ VL) n with (blocks, (kk,vv)) =>
+          Generate RI (v, k, z) (Z.of_nat ((32 * n)%nat)) 
+          = generate_algorithm_success (firstn (32 * n) (bitsToBytes (flatten (rev (map (@Vector.to_list _ 256) blocks)))))
                                        (bitsToBytes (@Vector.to_list _ 256 vv), bitsToBytes (@Vector.to_list _ 256 kk), z+1)
     end.
 Proof.
-  remember (GenUpdate_original_Zlist (k,v) (S n)) as g. symmetry in Heqg; destruct g as [a [b c]].
-  specialize (GenerateCorrect RI k v z n Z). rewrite Heqg; intros HH; rewrite HH.
-  specialize (GenUpdate_original_Zlist_Blist _ _ (S n) K V); rewrite Heqg; intros.
+  remember (GenUpdate_original_Zlist (k,v) n) as g. symmetry in Heqg; destruct g as [a [b c]].
+  specialize (GenerateCorrect RI k v z n Z N). rewrite Heqg; intros HH; rewrite HH.
+  specialize (GenUpdate_original_Zlist_Blist _ _ n K V); rewrite Heqg; intros.
   remember ( GenUpdate_original_Bvec
-    (of_list_length (bytesToBits k) KL, of_list_length (bytesToBits v) VL)
-    (S n)) as p. destruct p as [blocks [kk vv]]; symmetry in Heqp. 
+    (of_list_length (bytesToBits k) KL, of_list_length (bytesToBits v) VL) n) as p.
+  destruct p as [blocks [kk vv]]; symmetry in Heqp. 
   specialize (GenUpdate_original_Blist_Bvec (of_list_length (bytesToBits k) KL)
-                 (of_list_length (bytesToBits v) VL) (S n)).
+                 (of_list_length (bytesToBits v) VL) n).
   simpl. simpl in Heqp. rewrite Heqp; clear Heqp. simpl in H.
   rewrite ! HMAC_equivalence.of_length_proof_irrel. rewrite H; clear H. intros. inv H.
   apply  GenUpdate_original_Zlist_isbyteZ in Heqg; trivial. destruct Heqg as [isbyteA [isbyteVV isbyteKK]].
@@ -512,44 +569,166 @@ Proof.
   - rewrite ! bytes_bits_bytes_id; trivial.
 Qed.
 
-Lemma Generate_ok' RI k v z n (Z: (z<=RI)%Z) l kk vv zz 
+Lemma Generate_ok' RI k v z n (Z: (z<=RI)%Z) l kk vv zz (N:(0<n)%nat)
     (K: Forall isbyteZ k) (KL: length (bytesToBits k) = 256%nat) (V:Forall isbyteZ v) (VL:length (bytesToBits v) = 256%nat):
-    Generate RI (v, k, z) (Z.of_nat ((32 * n +1)%nat)) = generate_algorithm_success l (kk,vv, zz) ->
-    match GenUpdate_original_core (of_list_length _ KL, of_list_length _ VL) (S n) with (blocks, kv) =>
+    Generate RI (v, k, z) (Z.of_nat ((32 * n)%nat)) = generate_algorithm_success l (kk,vv, zz) ->
+    match GenUpdate_original_core (of_list_length _ KL, of_list_length _ VL) n with (blocks, kv) =>
     zz=z+1 /\ 
     bitsToBytes (@Vector.to_list _ 256 (fst kv)) = vv /\ 
     bitsToBytes (@Vector.to_list _ 256 (snd kv)) = kk /\
-          l = firstn (32 * n + 1) (bitsToBytes (flatten (map (@Vector.to_list _ 256) blocks)))
+          l = firstn (32 * n) (bitsToBytes (flatten (map (@Vector.to_list _ 256) blocks)))
     end.
 Proof. intros.
-  specialize (Generate_Bvec_ok' RI k v z n Z l kk vv zz K KL V VL H); clear H; intros.
+  specialize (Generate_Bvec_ok' RI k v z n Z l kk vv zz N K KL V VL H); clear H; intros.
   remember (GenUpdate_original_Bvec
         (of_list_length (bytesToBits k) KL,
-        of_list_length (bytesToBits v) VL) (S n)) as p; symmetry in Heqp; destruct p as [blocks state]. 
+        of_list_length (bytesToBits v) VL) n) as p; symmetry in Heqp; destruct p as [blocks state]. 
   specialize (GenUpdate_original_Bvec_correct
                (of_list_length (bytesToBits k) KL,
-                of_list_length (bytesToBits v) VL) (S n)). 
+                of_list_length (bytesToBits v) VL) n). 
   rewrite Heqp; clear Heqp; intros Q; rewrite Q, map_rev; apply H.
 Qed.
-Lemma Generate_ok RI k v z n (Z: (z<=RI)%Z) 
+Lemma Generate_ok RI k v z n (Z: (z<=RI)%Z) (N:(0<n)%nat)
               (K: Forall isbyteZ k) (KL: length (bytesToBits k) = 256%nat)
               (V:Forall isbyteZ v) (VL:length (bytesToBits v) = 256%nat):
-    match GenUpdate_original_core (of_list_length _ KL, of_list_length _ VL) (S n) with (blocks, (kk,vv)) =>
-          Generate RI (v, k, z) (Z.of_nat ((32 * n +1)%nat)) 
-          = generate_algorithm_success (firstn (32 * n + 1) (bitsToBytes (flatten (map (@Vector.to_list _ 256) blocks))))
+    match GenUpdate_original_core (of_list_length _ KL, of_list_length _ VL) n with (blocks, (kk,vv)) =>
+          Generate RI (v, k, z) (Z.of_nat ((32 * n)%nat)) 
+          = generate_algorithm_success (firstn (32 * n) (bitsToBytes (flatten (map (@Vector.to_list _ 256) blocks))))
                                        (bitsToBytes (@Vector.to_list _ 256 vv), bitsToBytes (@Vector.to_list _ 256 kk), z+1)
     end.
 Proof.
   remember (GenUpdate_original_Bvec
         (of_list_length (bytesToBits k) KL,
-        of_list_length (bytesToBits v) VL) (S n)) as p; destruct p as [blocks [kk vv]]; symmetry in Heqp.
+        of_list_length (bytesToBits v) VL) n) as p; destruct p as [blocks [kk vv]]; symmetry in Heqp.
   
   specialize (GenUpdate_original_Bvec_correct (of_list_length (bytesToBits k) KL,
-         of_list_length (bytesToBits v) VL) (S n)). rewrite Heqp. 
+         of_list_length (bytesToBits v) VL) n). rewrite Heqp. 
   intros Q; rewrite Q; clear Q.
-  specialize (Generate_Bvec_ok RI k v z n Z K KL V VL). rewrite Heqp; clear Heqp.
+  specialize (Generate_Bvec_ok RI k v z n Z N K KL V VL). rewrite Heqp; clear Heqp.
   intros W; rewrite W, map_rev; trivial. 
 Qed.
+
+Require Import hmacdrbg.entropy.
+Require Import hmacdrbg.HMAC_DRBG_common_lemmas.
+
+Lemma Bridge s I n bytes J ss (M: mbedtls_HMAC256_DRBG_generate_function s I n [] = ENTROPY.success (bytes, J) ss):
+  match I with HMAC256DRBGabs K V reseed_counter entropy_len prediction_resistance reseed_interval =>
+  reseed_counter <= reseed_interval -> prediction_resistance = false ->
+  match J with (ws,sstrength,prflag) =>
+  s=ss /\ Generate reseed_interval (V,K,reseed_counter) n = DRBG_functions.generate_algorithm_success bytes ws
+  end end.
+Proof. destruct I. destruct J as [[ws sstrength] prf].
+Transparent Generate. simpl. Opaque Generate. simpl in M.
+remember (n >? 1024) as d; destruct d; try discriminate.
+rewrite andb_negb_r in M. intros; subst.
+apply Zgt_is_gt_bool_f in H. rewrite H.
+remember (HMAC_DRBG_algorithms.HMAC_DRBG_generate_helper_Z HMAC256 key V n) as p; destruct p.
+unfold HMAC256_DRBG_functional_prog.HMAC256_DRBG_generate_algorithm in M; simpl in M.
+rewrite H, <- Heqp in M. inv M; split; trivial.
+Qed.
+
+(*The function occurring in the VST spec of mbedtls' random function ie no additional input*) 
+Definition mbedlts_generate s I n :=
+   match mbedtls_HMAC256_DRBG_generate_function s I n [] 
+   with ENTROPY.success (bytes, J) ss =>
+          match J with ((((VV, KK), RC), _), PR) =>
+            Some (bytes, ss, HMAC256DRBGabs KK VV RC (hmac256drbgabs_entropy_len I) PR 
+                                 (hmac256drbgabs_reseed_interval I))
+          end
+      | _ => None  
+   end.
+
+Lemma Bridge' s I n bytes F ss (M: mbedlts_generate s I n = Some(bytes, ss, F)):
+  match I with HMAC256DRBGabs K V reseed_counter entropy_len prediction_resistance reseed_interval =>
+  reseed_counter <= reseed_interval -> prediction_resistance = false ->
+  match F with HMAC256DRBGabs KK VV rc _ _ _ =>
+  s=ss /\ rc=reseed_counter+1 /\
+  Generate reseed_interval (V,K,reseed_counter) n = DRBG_functions.generate_algorithm_success bytes ((VV,KK), rc)
+  end end.
+Proof. destruct I. destruct F. Transparent Generate. simpl. Opaque Generate.
+unfold mbedlts_generate in M. simpl in M.
+remember (n >? 1024) as d; destruct d; try discriminate.
+rewrite andb_negb_r in M. intros; subst.
+apply Zgt_is_gt_bool_f in H.  rewrite H.
+remember (HMAC_DRBG_algorithms.HMAC_DRBG_generate_helper_Z HMAC256 key V n) as p; destruct p.
+unfold HMAC256_DRBG_functional_prog.HMAC256_DRBG_generate_algorithm in M; simpl in M.
+rewrite H, <- Heqp in M. inv M; auto. 
+Qed.
+
+Lemma Bridge_ok' s I (n:nat) bytes F ss (M: mbedlts_generate s I (32 * Z.of_nat n) = Some(bytes, ss, F)) (N:(0 < n)%nat):
+  match I with HMAC256DRBGabs k v reseed_counter entropy_len prediction_resistance reseed_interval =>
+  reseed_counter <= reseed_interval -> prediction_resistance = false ->
+  forall (K: Forall isbyteZ k) (KL: length (bytesToBits k) = 256%nat) (V:Forall isbyteZ v) (VL:length (bytesToBits v) = 256%nat),
+  match F with HMAC256DRBGabs KK VV rc _ _ _ =>
+  s=ss /\ rc=reseed_counter+1 /\
+    match GenUpdate_original_core (Blist.of_list_length _ KL, Blist.of_list_length _ VL) n with (blocks, kv) =>
+    bitsToBytes (@Vector.to_list _ 256 (fst kv)) = KK /\ 
+    bitsToBytes (@Vector.to_list _ 256 (snd kv)) = VV /\
+          bytes = firstn (32 * n) (bitsToBytes (Fold.flatten (map (@Vector.to_list _ 256) blocks)))
+    end
+  end end.
+Proof.
+ specialize (Bridge' _ _ _ _ _ _ M); destruct I; intros.
+ specialize (H H0 H1). destruct F. destruct H as [HH1 [HH2 HH3]].
+ split; trivial. split; trivial.
+ specialize (Generate_ok' reseed_interval key V reseed_counter n H0 bytes V1 key0 reseed_counter0).
+ rewrite Nat2Z.inj_mul. simpl. rewrite HH3.
+ clear HH3 M.
+ intros ZZ. specialize (ZZ N K KL V0 VL (eq_refl _)).
+ remember (HMAC_DRBG_nonadaptive.Gen_loop HMAC_Bvec
+           (Blist.of_list_length (bytesToBits key) KL)
+           (Blist.of_list_length (bytesToBits V) VL) n) as q.
+ destruct q. destruct ZZ as [_ ZZ].   apply ZZ.
+Qed.
+
+Lemma GenUpdate_original_core_length: forall n state l m
+  (G: GenUpdate_original_core state n = (l,m)),
+   length l = n%nat.
+Proof. induction n; destruct state; simpl; intros. 
++ inv G. simpl; omega.
++ remember (HMAC_DRBG_nonadaptive.Gen_loop HMAC_Bvec b
+           (HMAC_Bvec b (HMAC_DRBG_nonadaptive.to_list b0)) n) as q.
+  destruct q.  inv G. simpl. symmetry in Heqq. apply Genloop_Zlength_blocks in Heqq. 
+  rewrite (Zlength_correct l0) in Heqq. apply Nat2Z.inj in Heqq. subst; trivial.
+Qed.
+
+Lemma fold_vector_length: forall l m,
+fold_left
+  (fun (acc : nat) (a : Vector.t bool 256) =>
+   (acc + Datatypes.length (Vector.to_list a))%nat) l m =
+  (m + Datatypes.length l * 256)%nat.
+Proof. induction l; simpl; intros. + omega.
++ rewrite IHl, Blist.to_list_length; clear IHl. omega.
+Qed. 
+
+Lemma mbedlts_generate_Bridge s I (n:nat) bytes F ss (M: mbedlts_generate s I (32 * Z.of_nat n) = Some(bytes, ss, F)) (N:(0 < n)%nat):
+  match I with HMAC256DRBGabs k v reseed_counter entropy_len prediction_resistance reseed_interval =>
+  reseed_counter <= reseed_interval -> prediction_resistance = false ->
+  forall (K: Forall isbyteZ k) (KL: length (bytesToBits k) = 256%nat) (V:Forall isbyteZ v) (VL:length (bytesToBits v) = 256%nat),
+  match F with HMAC256DRBGabs KK VV rc _ _ _ =>
+  s=ss /\ rc=reseed_counter+1 /\
+    match GenUpdate_original_core (Blist.of_list_length _ KL, Blist.of_list_length _ VL) n with (blocks, kv) =>
+    bitsToBytes (@Vector.to_list _ 256 (fst kv)) = KK /\ 
+    bitsToBytes (@Vector.to_list _ 256 (snd kv)) = VV /\
+          bytes = (bitsToBytes (Fold.flatten (map (@Vector.to_list _ 256) blocks)))
+    end
+  end end.
+Proof.
+ specialize (Bridge_ok' _ _ _ _ _ _ M N); destruct I; intros.
+ specialize (H H0 H1 K KL V0 VL). destruct F. destruct H as [HH1 [HH2 HH3]].
+ split; trivial. split; trivial.
+ remember (GenUpdate_original_core
+          (Blist.of_list_length (bytesToBits key) KL,
+          Blist.of_list_length (bytesToBits V) VL) n) as q. destruct q.
+ rewrite sublist.firstn_same in HH3. trivial.
+ symmetry in Heqq. apply GenUpdate_original_core_length in Heqq.
+ assert (Datatypes.length (bitsToBytes (Fold.flatten (map Vector.to_list l))) = (32*n)%nat).
+ apply bitsToBytes_len_gen. rewrite CompFold.length_flatten. simpl. rewrite CompFold.fold_left_map_eq.
+ subst n. rewrite fold_vector_length. simpl. rewrite (mult_comm 32). rewrite <- mult_assoc.
+ replace (32*8)%nat with 256%nat. trivial. omega.
+ rewrite H. omega.
+Qed.  
+
 (*
 Require Import fcf.FCF.
 Definition GenUpdate_original_refactored (state : KV 256) (n : nat) :
